New arrangement of encoding/decoding:
EncodeTheory
+ Well-formed encoders
+ Encoders for primitive types

DecodeTheory
+ Well-formed decoders
+ Decoders defined as the inverse of encoders,
+ Decoders for primitive types

CoderTheory
+ Well-formed encoder/decoder pairs
+ Theorem that being well-formed satisfies conditions required by HolBddLib.

src/Boolify/src/CoderScript.sml
@@ -1,14 +1,16 @@
 (*===========================================================================*)
-(* Showing Encoding and Decoding to be inverse operations.                   *)
+(* Defining Decoders to be inverse Encoders                                  *)
 (*===========================================================================*)
 
 (* Interactive mode
-app load ["rich_listTheory", "EncodeTheory", "normalForms"];
+app load
+["bossLib", "rich_listTheory", "EncodeTheory", "DecodeTheory", "normalForms",
+ "metisLib"];
 *)
 
 open HolKernel boolLib Parse bossLib pairTheory pairTools
-     arithmeticTheory listTheory rich_listTheory EncodeTheory
-     mesonLib optionTheory normalForms combinTheory;
+     arithmeticTheory listTheory rich_listTheory EncodeTheory DecodeTheory
+     metisLib optionTheory normalForms combinTheory;
 
 val _ = new_theory "Coder";
 
@@ -26,199 +28,19 @@ val Know = Q_TAC KNOW_TAC;
 val REVERSE = Tactical.REVERSE;
 
 (*---------------------------------------------------------------------------
-     decode turns a decoding parser of type
-       bool list -> ('a # bool list) option
-     into a straight function of type
-       bool list -> 'a
-
-     domain parser identifies the set of bool lists where it is valid
-     to apply decode parser (i.e., any bool list l such that parser l
-     results in a successful parse with no bools remaining: SOME (t, []))
+     Well-formed encoder/decoder pairs.
  ---------------------------------------------------------------------------*)
 
-val decode_def = Define `decode f = FST o THE o f`;
-
-local
-  val th =prove
-  (``?d. !f x. x IN d f = ?y. f x = SOME (y, [])``,
-   Q.EXISTS_TAC `\f x. ?y. f x = SOME (y, [])` ++
-   SIMP_TAC bool_ss [IN_DEF]);
-in
-  val domain_def =
-    Definition.new_specification ("domain_def", ["domain"], th);
-  val _ = add_const "domain";
-end;
+val wf_coder_def =
+ Define `wf_coder p (e : 'a -> bool list) d = (!x. p x ==> (d (e x) = x))`;
 
 (*---------------------------------------------------------------------------
-     Well-formed decoders.
+     Well-formed coders occur naturally from use of enc2dec.
  ---------------------------------------------------------------------------*)
-
-val wf_pdecoder_def = Define
-  `wf_pdecoder p (d : bool list -> ('a # bool list) option) =
-   !x.
-     if p x then (?a. !b c. (d b = SOME (x, c)) = (b = APPEND a c))
-     else !a b. ~(d a = SOME (x, b))`;
-
-(*---------------------------------------------------------------------------
-     Functions to transform well-formed encoders to well-formed decoders,
-     and vice versa.
- ---------------------------------------------------------------------------*)
-
-val enc2dec_def = Define
-  `enc2dec p e (l : bool list) =
-   if ?x t. p (x : 'a) /\ (l = APPEND (e x) t)
-   then SOME (@(x, t). p x /\ (l = APPEND (e x) t))
-   else NONE`;
-
-val dec2enc_def = Define
-  `dec2enc (d : bool list -> ('a # bool list) option) x =
-   @l. d l = SOME (x, [])`;
-
-(*---------------------------------------------------------------------------
-     Proofs that the transformation functions are mutually inverse.
- ---------------------------------------------------------------------------*)
-
-val enc2dec_none = store_thm
-  ("enc2dec_none",
-   ``!p e l. (enc2dec p e l = NONE) = (!x t. p x ==> ~(l = APPEND (e x) t))``,
-   RW_TAC std_ss [enc2dec_def] ++
-   PROVE_TAC []);
-
-val enc2dec_some = store_thm
-  ("enc2dec_some",
-   ``!p e l x t.
-       wf_pencoder p e ==>
-       ((enc2dec p e l = SOME (x, t)) = p x /\ (l = APPEND (e x) t))``,
-   REVERSE (RW_TAC std_ss [enc2dec_def]) >> PROVE_TAC [] ++
-   ONCE_REWRITE_TAC [GSYM (ONCE_DEPTH_CONV ETA_CONV ``@p. q p``)] ++
-   SELECT_TAC ++
-   RW_TAC std_ss [UNCURRY] ++
-   Cases_on `p'` ++
-   EQ_TAC >>
-   (DISCH_THEN (fn th => POP_ASSUM MP_TAC THEN SUBST1_TAC th) ++
-    SIMP_TAC std_ss [] ++
-    DISCH_THEN MATCH_MP_TAC ++
-    PROVE_TAC [FST, SND]) ++
-   POP_ASSUM MP_TAC ++
-   MATCH_MP_TAC
-   (PROVE [] ``(z ==> x) /\ (y ==> z ==> t) ==> (x ==> y) ==> z ==> t``) ++
-   CONJ_TAC >> PROVE_TAC [FST, SND] ++
-   SIMP_TAC std_ss [] ++
-   REPEAT (DISCH_THEN STRIP_ASSUME_TAC) ++
-   Suff `q = x` >> PROVE_TAC [APPEND_11] ++
-   FULL_SIMP_TAC std_ss [wf_pencoder_def] ++
-   PROVE_TAC [IS_PREFIX_APPEND1, IS_PREFIX_APPEND2, IS_PREFIX_REFL]);
-
-val wf_enc2dec = store_thm
-  ("wf_enc2dec",
-   ``!p e. wf_pencoder p e ==> wf_pdecoder p (enc2dec p e)``,
-   RW_TAC std_ss [wf_pdecoder_def, enc2dec_some] ++
-   PROVE_TAC [APPEND_NIL]);
-
-val dec2enc_some = store_thm
-  ("dec2enc_some",
-   ``!p d x l.
-       wf_pdecoder p d ==>
-       ((dec2enc d x = l) /\ p x = (d l = SOME (x, [])))``,
-   RW_TAC std_ss [dec2enc_def] ++
-   SELECT_TAC ++
-   RW_TAC std_ss [] ++
-   EQ_TAC >>
-   (RW_TAC std_ss [] ++
-    Q.PAT_ASSUM `X ==> Y` MATCH_MP_TAC ++
-    FULL_SIMP_TAC std_ss [wf_pdecoder_def] ++
-    PROVE_TAC [APPEND_NIL]) ++
-   POP_ASSUM MP_TAC ++
-   MATCH_MP_TAC
-   (PROVE [] ``(z ==> x) /\ (y ==> z ==> t) ==> (x ==> y) ==> z ==> t``) ++
-   CONJ_TAC >> PROVE_TAC [] ++
-   POP_ASSUM MP_TAC ++
-   SIMP_TAC std_ss [wf_pdecoder_def] ++
-   DISCH_THEN (MP_TAC o Q.SPEC `x`) ++
-   REVERSE (Cases_on `p x`) >> PROVE_TAC [] ++
-   ASM_REWRITE_TAC [] ++
-   DISCH_THEN (CHOOSE_THEN MP_TAC) ++
-   RW_TAC std_ss []);
-
-val decode_dec2enc = store_thm
-  ("decode_dec2enc",
-   ``!p d x.
-       wf_pdecoder p d /\ p x ==> (d (dec2enc d x) = SOME (x, []))``,
-   PROVE_TAC [dec2enc_some]);
-
-val decode_dec2enc_append = store_thm
-  ("decode_dec2enc_append",
-   ``!p d x t.
-       wf_pdecoder p d /\ p x ==>
-       (d (APPEND (dec2enc d x) t) = SOME (x, t))``,
-   RW_TAC std_ss [] ++
-   MP_TAC (Q.SPECL [`p`, `d`, `x`] decode_dec2enc) ++
-   RW_TAC std_ss [] ++
-   FULL_SIMP_TAC std_ss [wf_pdecoder_def] ++
-   Q.PAT_ASSUM `!x. P x` (MP_TAC o Q.SPEC `x`) ++
-   RW_TAC std_ss [] ++
-   RW_TAC std_ss [] ++
-   RES_TAC ++
-   RW_TAC std_ss [APPEND_NIL]);
-
-val wf_dec2enc = store_thm
-  ("wf_dec2enc",
-   ``!p d. wf_pdecoder p d ==> wf_pencoder p (dec2enc d)``,
-   RW_TAC std_ss [wf_pencoder_def] ++
-   MP_TAC (Q.SPECL [`p`, `d`] wf_pdecoder_def) ++
-   ASM_REWRITE_TAC [] ++
-   DISCH_THEN (fn th => MP_TAC (Q.SPEC `x` th) THEN MP_TAC (Q.SPEC `y` th)) ++
-   RW_TAC std_ss [] ++
-   MP_TAC (Q.SPECL [`p`, `d`, `x`] decode_dec2enc) ++
-   MP_TAC (Q.SPECL [`p`, `d`, `y`] decode_dec2enc) ++
-   RW_TAC std_ss [APPEND_NIL] ++
-   POP_ASSUM MP_TAC ++
-   POP_ASSUM MP_TAC ++
-   POP_ASSUM (CHOOSE_THEN MP_TAC o REWRITE_RULE [IS_PREFIX_APPEND]) ++
-   RW_TAC std_ss [GSYM APPEND_ASSOC] ++
-   POP_ASSUM (MP_TAC o Q.SPECL [`APPEND (dec2enc d y) l`, `[]`]) ++
-   POP_ASSUM (MP_TAC o Q.SPECL [`APPEND (dec2enc d y) l`, `l`]) ++
-   RW_TAC std_ss [APPEND_NIL]);
-
-val dec2enc_enc2dec = store_thm
-  ("dec2enc_enc2dec",
-   ``!p e x. wf_pencoder p e /\ p x ==> (dec2enc (enc2dec p e) x = e x)``,
-   RW_TAC std_ss [] ++
-   MP_TAC (Q.SPECL [`p`, `e`] wf_enc2dec) ++
-   RW_TAC std_ss [dec2enc_some] ++
-   MP_TAC (Q.SPECL [`p`, `enc2dec p e`, `x`, `e x`] dec2enc_some) ++
-   RW_TAC std_ss [enc2dec_some, APPEND_NIL]);
-
-val enc2dec_dec2enc = store_thm
-  ("enc2dec_dec2enc",
-   ``!p d. wf_pdecoder p d ==> (enc2dec p (dec2enc d) = d)``,
-   RW_TAC std_ss [] ++
-   MATCH_MP_TAC EQ_EXT ++
-   Q.X_GEN_TAC `l` ++
-   MP_TAC (Q.SPECL [`p`, `d`] wf_dec2enc) ++
-   RW_TAC std_ss [] ++
-   Cases_on `d l` <<
-   [RW_TAC std_ss [enc2dec_none] ++
-    STRIP_TAC ++
-    RW_TAC std_ss [] ++
-    Q.PAT_ASSUM `X = Y` MP_TAC ++
-    PROVE_TAC [NOT_SOME_NONE, decode_dec2enc_append],
-    Cases_on `x` ++
-    ASM_SIMP_TAC std_ss [enc2dec_some] ++
-    MATCH_MP_TAC (PROVE [] ``x /\ (x ==> y) ==> x /\ y``) ++
-    RW_TAC std_ss [] >> PROVE_TAC [wf_pdecoder_def] ++
-    MP_TAC (Q.SPECL [`p`, `d`] wf_pdecoder_def) ++
-    ASM_REWRITE_TAC [] ++
-    DISCH_THEN (MP_TAC o Q.SPEC `q`) ++
-    RW_TAC std_ss [] ++
-    RES_TAC ++
-    RW_TAC std_ss [APPEND_11] ++
-    Suff `d a = SOME (q, [])` >> PROVE_TAC [dec2enc_some] ++
-    RW_TAC std_ss [APPEND_NIL]]);
 
 val decode_encode = store_thm
   ("decode_encode",
-   ``!p e x. wf_pencoder p e /\ p x ==> (decode (enc2dec p e) (e x) = x)``,
+   ``!p e x. wf_encoder p e /\ p x ==> (decode (enc2dec p e) (e x) = x)``,
    RW_TAC std_ss [] ++
    Cases_on `enc2dec p e (e x)` >>
    (POP_ASSUM MP_TAC ++
@@ -228,164 +50,68 @@ val decode_encode = store_thm
    Cases_on `x'` ++
    SIMP_TAC std_ss [decode_def, o_THM] ++
    RW_TAC std_ss [enc2dec_some] ++
-   MP_TAC (Q.SPECL [`p`, `e`] wf_pencoder_def) ++
+   MP_TAC (Q.SPECL [`p`, `e`] wf_encoder_def) ++
    RW_TAC std_ss [] ++
    Suff `IS_PREFIX (e x) (e q)` >> PROVE_TAC [] ++
    PROVE_TAC [IS_PREFIX_APPEND]);
 
-val encode_decode = store_thm
-  ("encode_decode",
-   ``!p e. !l :: domain (enc2dec p e).
-       wf_pencoder p e ==> (e (decode (enc2dec p e) l) = l)``,
-   RW_TAC std_ss [RES_FORALL_DEF, domain_def, decode_def, o_THM] ++
-   RW_TAC std_ss [] ++
-   Q.PAT_ASSUM `X = Y` MP_TAC ++
-   RW_TAC std_ss [enc2dec_some, APPEND_NIL]);
+val wf_coder = store_thm
+  ("wf_coder",
+   ``!p e. wf_encoder p e ==> wf_coder p e (decode (enc2dec p e))``,
+   RW_TAC std_ss [wf_coder_def, decode_encode]);
+
+val wf_coder_op = store_thm
+  ("wf_coder_op",
+   ``!p e f.
+       wf_encoder p e /\ (!x. p x ==> (e x = f x)) ==>
+       wf_coder p e (decode (enc2dec p f))``,
+   RW_TAC std_ss [wf_coder_def]
+   ++ HO_METIS_TAC [decode_encode, wf_encoder_eq]);
 
 (*---------------------------------------------------------------------------
-     We define decoders in terms of encoders.
+     Boolean coders
  ---------------------------------------------------------------------------*)
 
-val decode_bool_def = Define `decode_bool = enc2dec total encode_bool`;
-
-val decode_list_def = Define
-  `decode_list p d = enc2dec p (encode_list (dec2enc d))`;
+val wf_coder_bool = store_thm
+  ("wf_coder_bool",
+   ``wf_coder total encode_bool decode_bool``,
+   RW_TAC std_ss [wf_encode_bool, decode_bool_def, wf_coder, dec_bool_def]);
 
 (*---------------------------------------------------------------------------
-     decoders are well-formed and satisfy natural recursion equations.
+     List coders
  ---------------------------------------------------------------------------*)
 
-val wf_decode_bool = store_thm
-  ("wf_decode_bool",
-   ``wf_pdecoder total decode_bool``,
-   RW_TAC std_ss [decode_bool_def, wf_enc2dec, wf_encoder, wf_encode_bool]);
+val wf_coder_list = store_thm
+  ("wf_coder_list",
+   ``!p (e : 'a -> bool list).
+       wf_encoder p e ==>
+       wf_coder (EVERY p) (encode_list e)
+       (decode_list (EVERY p) (enc2dec p e))``,
+   RW_TAC std_ss [decode_list_def, dec_list_def]
+   ++ MATCH_MP_TAC wf_coder_op
+   ++ RW_TAC std_ss [wf_encode_list]
+   ++ Induct_on `x`
+   ++ RW_TAC std_ss [encode_list_def, EVERY_DEF, dec2enc_enc2dec]);
 
-val decode_encode_bool = store_thm
-  ("decode_encode_bool",
-   ``!x. decode decode_bool (encode_bool x) = x``,
-   RW_TAC std_ss
-   [decode_encode, decode_bool_def, wf_encoder, wf_encode_bool, total_def]);
+(*---------------------------------------------------------------------------
+     Tree coders
+ ---------------------------------------------------------------------------*)
 
-val encode_decode_bool = store_thm
-  ("encode_decode_bool",
-   ``!l :: domain decode_bool. encode_bool (decode decode_bool l) = l``,
-   MP_TAC (Q.ISPECL [`total : bool -> bool`, `encode_bool`] encode_decode) ++
-   RW_TAC std_ss [decode_bool_def, wf_encoder, wf_encode_bool, total_def]);
-
-val decode_bool = store_thm
-  ("decode_bool",
-   ``decode_bool l = case l of [] -> NONE || (h :: t) -> SOME (h, t)``,
-   REPEAT CASE_TAC ++
-   RW_TAC std_ss
-   [decode_bool_def, enc2dec_none, enc2dec_some, encode_bool_def,
-    APPEND, wf_encode_bool, wf_encoder, total_def]);
-
-val wf_decode_list = store_thm
-  ("wf_decode_list",
-   ``!p d.
-       wf_pdecoder p d ==> wf_pdecoder (EVERY p) (decode_list (EVERY p) d)``,
-   RW_TAC std_ss [decode_list_def] ++
-   PROVE_TAC [wf_dec2enc, wf_enc2dec, wf_pencode_list]);
-
-(* in progress ***
-val decode_encode_list = store_thm
-  ("decode_encode_list",
-   ``!p e x.
-       wf_pencoder p e /\ EVERY p x ==>
-       (decode (decode_list (EVERY p) (enc2dec p e)) (encode_list e x) = x)``,
-   RW_TAC std_ss [decode_encode, wf_pencode_list]
-decode_bool_def, wf_encoder, wf_encode_bool, total_def]);
-
-val encode_decode_bool = store_thm
-  ("encode_decode_bool",
-   ``!l :: domain decode_bool. encode_bool (decode decode_bool l) = l``,
-   MP_TAC (Q.ISPECL [`total : bool -> bool`, `encode_bool`] encode_decode) ++
-   RW_TAC std_ss [decode_bool_def, wf_encoder, wf_encode_bool, total_def]);
-*)
-
-val decode_list = store_thm
-  ("decode_list",
-   ``wf_pdecoder p d ==>
-     (decode_list (EVERY p) d l =
-      case l of [] -> NONE
-      || (T :: t) ->
-         (case d t of NONE -> NONE
-          || SOME (x, t') ->
-             (case decode_list (EVERY p) d t' of NONE -> NONE
-              || SOME (xs, t'') -> SOME (x :: xs, t'')))
-      || (F :: t) -> SOME ([], t))``,
-   (REPEAT CASE_TAC ++
-    RW_TAC std_ss [decode_list_def, enc2dec_none]) <<
-   [Cases_on `x` ++
-    RW_TAC std_ss [encode_list_def, APPEND],
-    Cases_on `x` ++
-    POP_ASSUM MP_TAC ++
-    RW_TAC std_ss [encode_list_def, APPEND, GSYM APPEND_ASSOC, EVERY_DEF] ++
-    POP_ASSUM (K ALL_TAC) ++
-    Q.SPEC_TAC (`APPEND (encode_list (dec2enc d) t'') t'`, `l`) ++
-    REPEAT STRIP_TAC ++
-    RW_TAC std_ss [] ++
-    MP_TAC (Q.SPECL [`p`, `d`] wf_pdecoder_def) ++
-    RW_TAC std_ss [] ++
-    Q.EXISTS_TAC `h` ++
-    RW_TAC std_ss [] ++
-    PROVE_TAC [decode_dec2enc_append, NOT_SOME_NONE],
-    Cases_on `x` ++
-    POP_ASSUM MP_TAC ++
-    RW_TAC std_ss [encode_list_def, APPEND, GSYM APPEND_ASSOC, EVERY_DEF] ++
-    STRIP_TAC ++
-    RW_TAC std_ss [] ++
-    Q.PAT_ASSUM `X = SOME Y` MP_TAC ++
-    MP_TAC (Q.SPECL [`p`, `d`, `h`] decode_dec2enc_append) ++
-    ASM_SIMP_TAC std_ss [] ++
-    DISCH_THEN (K ALL_TAC) ++
-    PURE_REWRITE_TAC [GSYM DE_MORGAN_THM] ++
-    STRIP_TAC ++
-    RW_TAC std_ss [] ++
-    Q.PAT_ASSUM `X = Y` MP_TAC ++
-    RW_TAC std_ss [decode_list_def, enc2dec_none] ++
-    PROVE_TAC [],
-    Know `wf_pdecoder (EVERY p) (decode_list (EVERY p) d)` >>
-    PROVE_TAC [wf_decode_list] ++
-    STRIP_TAC ++
-    Know `wf_pencoder p (dec2enc d)` >> PROVE_TAC [wf_dec2enc] ++
-    STRIP_TAC ++
-    Know `wf_pencoder (EVERY p) (encode_list (dec2enc d))` >>
-    PROVE_TAC [wf_pencode_list] ++
-    STRIP_TAC ++
-    ASM_SIMP_TAC std_ss [enc2dec_some, encode_list_def, APPEND] ++
-    MATCH_MP_TAC (PROVE [] ``x /\ (x ==> y) ==> x /\ y``) ++
-    CONJ_TAC >> PROVE_TAC [EVERY_DEF, wf_pdecoder_def, wf_decode_list] ++
-    RW_TAC std_ss [EVERY_DEF] ++
-    MP_TAC (Q.SPECL [`p`, `d`] wf_pdecoder_def) ++
-    ASM_SIMP_TAC std_ss [] ++
-    DISCH_THEN (MP_TAC o Q.SPEC `q`) ++
-    RW_TAC std_ss [] ++
-    RES_TAC ++
-    RW_TAC std_ss [GSYM APPEND_ASSOC] ++
-    Know `dec2enc d q = a` >> PROVE_TAC [APPEND_NIL, dec2enc_some] ++
-    RW_TAC std_ss [APPEND_11] ++
-    Q.PAT_ASSUM `!x. P x` (K ALL_TAC) ++
-    MP_TAC
-    (Q.ISPECL [`EVERY (p : 'a -> bool)`, `decode_list (EVERY p) d`]
-     wf_pdecoder_def) ++
-    ASM_SIMP_TAC std_ss [] ++
-    DISCH_THEN (MP_TAC o Q.SPEC `q'`) ++
-    RW_TAC std_ss [] ++
-    RES_TAC ++
-    RW_TAC std_ss [] ++
-    Q.PAT_ASSUM `!x. P x` (K ALL_TAC) ++
-    Q.PAT_ASSUM `X = Y` MP_TAC ++
-    ASM_SIMP_TAC std_ss [decode_list_def, enc2dec_some],
-    Know `wf_pdecoder (EVERY p) (decode_list (EVERY p) d)` >>
-    PROVE_TAC [wf_decode_list] ++
-    STRIP_TAC ++
-    Know `wf_pencoder p (dec2enc d)` >> PROVE_TAC [wf_dec2enc] ++
-    STRIP_TAC ++
-    Know `wf_pencoder (EVERY p) (encode_list (dec2enc d))` >>
-    PROVE_TAC [wf_pencode_list] ++
-    STRIP_TAC ++
-    ASM_SIMP_TAC std_ss [enc2dec_some, encode_list_def, APPEND, EVERY_DEF]]);
+val wf_coder_tree = store_thm
+  ("wf_coder_tree",
+   ``!p (e : 'a -> bool list).
+       wf_encoder p e ==>
+       wf_coder (lift_tree p) (encode_tree e)
+       (decode_tree (lift_tree p) (enc2dec p e))``,
+   RW_TAC std_ss [decode_tree_def, dec_tree_def]
+   ++ MATCH_MP_TAC wf_coder_op
+   ++ RW_TAC std_ss [wf_encode_tree]
+   ++ POP_ASSUM MP_TAC
+   ++ Q.SPEC_TAC (`x`, `t`)
+   ++ HO_MATCH_MP_TAC tree_ind
+   ++ RW_TAC std_ss [encode_tree_def, lift_tree_def, dec2enc_enc2dec, APPEND_11]
+   ++ Induct_on `ts`
+   ++ RW_TAC std_ss [MEM, encode_list_def, EVERY_DEF]);
 
 val _ = export_theory ();
 
